Dom/pureprimops (#10)
Co-authored-by: Julian Sutherland <julian.sutherland10@imperial.ac.uk>

src/YulPrimops.ec
@@ -1,10 +1,11 @@
 pragma Goals:printall.
 
-require import Logic Array.
+require import Array.
+require import Logic.
+require import PurePrimops.
+require import Real.
+require import Utils.
 require export UInt256 Memory.
-
-op calldata : uint256 array.
-(* op keccak256 : uint256 array -> uint256. *)
 
 module Primops = {
   var memory : mem
@@ -12,6 +13,7 @@ module Primops = {
 
   proc mload(idx : uint256) : uint256 = {
     (* _1 is the most significant byte *)
+    (* TODO replace definition with a direct call to op mload *)
     var _r1, _r2, _r3, _r4, _r5, _r6, _r7, _r8, _r9, _r10, _r11, _r12, _r13, _r14, _r15, _r16, _r17, _r18, _r19, _r20, _r21, _r22, _r23, _r24, _r25, _r26, _r27, _r28, _r29, _r30, _r31, _r32;
 
 
@@ -157,7 +159,7 @@ module Primops = {
     memory <- memory.[idx<-(val `&` W256.masklsb 8)];
   }
 
-  proc ret(retOff : uint256, retSize : uint256) : unit = {
+  proc evm_return(retOff : uint256, retSize : uint256) : unit = {
     (* TODO: Implement return *)
     return ();
   }
@@ -167,26 +169,8 @@ module Primops = {
     return W256.of_int 42;
   }
 
-  proc iszero(v : uint256) : uint256 = {
-    var ref;
-    if (v = W256.of_int 0) {
-      ref <- W256.one;
-    } else {
-      ref <- W256.zero;
-    }
-    return ref;
-  }
-
-  proc mulmod(a : uint256, b : uint256, n : uint256) : uint256 = {
-    return (a * b) %% n;
-  }
-
-  proc addmod(a : uint256, b : uint256, n : uint256) : uint256 = {
-    return (a + b) %% n;
-  }
-
-  proc keccak256(v : uint256) : uint256 = {
-    (* TODO: return sample from uniform distribution over uint256 *)
+  proc keccak256(off : uint256, size : uint256) : uint256 = {
+    (* TODO: relate to keccak_f *)
     return W256.zero;
   }
 
@@ -216,11 +200,440 @@ module Primops = {
     return succ;
   }
 
-  proc revert() : unit = {
+  proc revert(x : uint256, y : uint256) : unit = {
     reverted <- true;
   }
 
   proc calldataload(i : uint256) : uint256 = {
-    return calldata.[W256.to_uint i];
+    return PurePrimops.calldata.[W256.to_uint i];
   }
 }.
+
+theory ConcretePrimops.
+
+lemma mload_pspec (memory: mem) (idx: uint256):
+phoare [ Primops.mload :
+    arg = idx /\
+    Primops.memory = memory ==>
+      res = PurePrimops.mload memory idx /\
+      Primops.memory = memory
+    ] = 1%r.
+    proof.
+      progress.
+      proc.
+      wp.
+      skip.
+      progress.
+      rewrite /mload.
+      reflexivity.
+  qed.
+
+lemma mload_spec (memory: mem) (idx: uint256):
+hoare [ Primops.mload :
+    arg = idx /\
+    Primops.memory = memory ==>
+      res = PurePrimops.mload memory idx /\
+      Primops.memory = memory
+    ].
+    proof.
+      progress.
+      proc.
+      wp.
+      skip.
+      progress.
+      rewrite /mload.
+      reflexivity.
+  qed.
+    
+lemma mstore_pspec:
+    forall (memory: mem) (idx': uint256) (val': uint256),
+phoare [ Primops.mstore :
+    arg = (idx', val') /\
+    Primops.memory = memory ==>
+      Primops.memory = PurePrimops.mstore memory idx' val'
+    ] = 1%r.
+    proof.
+      progress.
+      proc.
+      wp.
+      skip.
+    move => &hr h_args.
+      have h_idx: idx{hr} = idx'.
+      smt.
+      have h_val: val{hr} = val'.
+      smt.
+      have h_mem: Primops.memory{hr} = memory.
+      smt.
+    move => x248 x240 x232 x224 x216 x208 x200 x192 x184 x176 x168 x160 x152 x144 x136 x128 x120 x112 x104 x96 x88 x80 x72 x64 x56 x48 x40 x32 x24 x16 x8.
+      apply PurePrimops.mstore_of_load_and_frame.
+      rewrite h_mem.
+      rewrite /mload.
+      rewrite h_idx.
+      rewrite {1} Map.get_set_sameE.
+      rewrite {1} get_set_offsets_neq; first trivial.
+      rewrite {1} Map.get_set_sameE.
+      rewrite masklsb_zero.
+      rewrite splitMask_zero.
+      rewrite shr_zero.
+      rewrite /x8.
+      rewrite splitMask2_shr_shl; first trivial.
+      rewrite splitMask_add.
+      do 2! (rewrite {1} get_set_offsets_neq; first trivial).
+      rewrite {1} Map.get_set_sameE.
+      rewrite /x16.
+      rewrite splitMask2_shr_shl; first trivial.
+      rewrite splitMask_add.
+      do 3! (rewrite {1} get_set_offsets_neq; first trivial).
+      rewrite {1} Map.get_set_sameE.
+      rewrite /x24.
+      rewrite splitMask2_shr_shl; first trivial.
+      rewrite splitMask_add.    
+      do 4! (rewrite {1} get_set_offsets_neq; first trivial).
+      rewrite {1} Map.get_set_sameE.
+      rewrite /x32.
+      rewrite splitMask2_shr_shl; first trivial.
+      rewrite splitMask_add.    
+      do 5! (rewrite {1} get_set_offsets_neq; first trivial).
+      rewrite {1} Map.get_set_sameE.
+      rewrite /x40.
+      rewrite splitMask2_shr_shl; first trivial.
+      rewrite splitMask_add.    
+      do 6! (rewrite {1} get_set_offsets_neq; first trivial).
+      rewrite {1} Map.get_set_sameE.
+      rewrite /x48.
+      rewrite splitMask2_shr_shl; first trivial.
+      rewrite splitMask_add.
+      do 7! (rewrite {1} get_set_offsets_neq; first trivial).
+      rewrite {1} Map.get_set_sameE.
+      rewrite /x56.
+      rewrite splitMask2_shr_shl; first trivial.
+      rewrite splitMask_add.
+      do 8! (rewrite {1} get_set_offsets_neq; first trivial).
+      rewrite {1} Map.get_set_sameE.
+      rewrite /x64.
+      rewrite splitMask2_shr_shl; first trivial.
+      rewrite splitMask_add.
+      do 9! (rewrite {1} get_set_offsets_neq; first trivial).
+      rewrite {1} Map.get_set_sameE.
+      rewrite /x72.
+      rewrite splitMask2_shr_shl; first trivial.
+      rewrite splitMask_add.
+      do 10! (rewrite {1} get_set_offsets_neq; first trivial).
+      rewrite {1} Map.get_set_sameE.
+      rewrite /x80.
+      rewrite splitMask2_shr_shl; first trivial.
+      rewrite splitMask_add.
+      do 11! (rewrite {1} get_set_offsets_neq; first trivial).
+      rewrite {1} Map.get_set_sameE.
+      rewrite /x88.
+      rewrite splitMask2_shr_shl; first trivial.
+      rewrite splitMask_add.
+      do 12! (rewrite {1} get_set_offsets_neq; first trivial).
+      rewrite {1} Map.get_set_sameE.
+      rewrite /x96.
+      rewrite splitMask2_shr_shl; first trivial.
+      rewrite splitMask_add.
+      do 13! (rewrite {1} get_set_offsets_neq; first trivial).
+      rewrite {1} Map.get_set_sameE.
+      rewrite /x104.
+      rewrite splitMask2_shr_shl; first trivial.
+      rewrite splitMask_add.
+      do 14! (rewrite {1} get_set_offsets_neq; first trivial).
+      rewrite {1} Map.get_set_sameE.
+      rewrite /x112.
+      rewrite splitMask2_shr_shl; first trivial.
+      rewrite splitMask_add.
+      do 15! (rewrite {1} get_set_offsets_neq; first trivial).
+      rewrite {1} Map.get_set_sameE.
+      rewrite /x120.
+      rewrite splitMask2_shr_shl; first trivial.
+      rewrite splitMask_add.
+      do 16! (rewrite {1} get_set_offsets_neq; first trivial).
+      rewrite {1} Map.get_set_sameE.
+      rewrite /x128.
+      rewrite splitMask2_shr_shl; first trivial.
+      rewrite splitMask_add.
+      do 17! (rewrite {1} get_set_offsets_neq; first trivial).
+      rewrite {1} Map.get_set_sameE.
+      rewrite /x136.
+      rewrite splitMask2_shr_shl; first trivial.
+      rewrite splitMask_add.
+      do 18! (rewrite {1} get_set_offsets_neq; first trivial).
+      rewrite {1} Map.get_set_sameE.
+      rewrite /x144.
+      rewrite splitMask2_shr_shl; first trivial.
+      rewrite splitMask_add.
+      do 19! (rewrite {1} get_set_offsets_neq; first trivial).
+      rewrite {1} Map.get_set_sameE.
+      rewrite /x152.
+      rewrite splitMask2_shr_shl; first trivial.
+      rewrite splitMask_add.
+      do 20! (rewrite {1} get_set_offsets_neq; first trivial).
+      rewrite {1} Map.get_set_sameE.
+      rewrite /x160.
+      rewrite splitMask2_shr_shl; first trivial.
+      rewrite splitMask_add.
+      do 21! (rewrite {1} get_set_offsets_neq; first trivial).
+      rewrite {1} Map.get_set_sameE.
+      rewrite /x168.
+      rewrite splitMask2_shr_shl; first trivial.
+      rewrite splitMask_add.
+      do 22! (rewrite {1} get_set_offsets_neq; first trivial).
+      rewrite {1} Map.get_set_sameE.
+      rewrite /x176.
+      rewrite splitMask2_shr_shl; first trivial.
+      rewrite splitMask_add.
+      do 23! (rewrite {1} get_set_offsets_neq; first trivial).
+      rewrite {1} Map.get_set_sameE.
+      rewrite /x184.
+      rewrite splitMask2_shr_shl; first trivial.
+      rewrite splitMask_add.
+      do 24! (rewrite {1} get_set_offsets_neq; first trivial).
+      rewrite {1} Map.get_set_sameE.
+      rewrite /x192.
+      rewrite splitMask2_shr_shl; first trivial.
+      rewrite splitMask_add.
+      do 25! (rewrite {1} get_set_offsets_neq; first trivial).
+      rewrite {1} Map.get_set_sameE.
+      rewrite /x200.
+      rewrite splitMask2_shr_shl; first trivial.
+      rewrite splitMask_add.
+      do 26! (rewrite {1} get_set_offsets_neq; first trivial).
+      rewrite {1} Map.get_set_sameE.
+      rewrite /x208.
+      rewrite splitMask2_shr_shl; first trivial.
+      rewrite splitMask_add.
+      do 27! (rewrite {1} get_set_offsets_neq; first trivial).
+      rewrite {1} Map.get_set_sameE.
+      rewrite /x216.
+      rewrite splitMask2_shr_shl; first trivial.
+      rewrite splitMask_add.
+      do 28! (rewrite {1} get_set_offsets_neq; first trivial).
+      rewrite {1} Map.get_set_sameE.
+      rewrite /x224.
+      rewrite splitMask2_shr_shl; first trivial.
+      rewrite splitMask_add.
+      do 29! (rewrite {1} get_set_offsets_neq; first trivial).
+      rewrite {1} Map.get_set_sameE.
+      rewrite /x232.
+      rewrite splitMask2_shr_shl; first trivial.
+      rewrite splitMask_add.
+      do 30! (rewrite {1} get_set_offsets_neq; first trivial).
+      rewrite {1} Map.get_set_sameE.
+      rewrite /x240.
+      rewrite splitMask2_shr_shl; first trivial.
+      rewrite splitMask_add.
+      do 31! (rewrite {1} get_set_offset; first trivial).
+      rewrite {1} Map.get_set_sameE.
+      rewrite /x248.
+      rewrite splitMask2_shr_shl; first trivial.
+      rewrite splitMask_add.
+      exact h_val.
+      rewrite /uint256_frame.
+    move => idx2 h_idx2.
+      rewrite h_idx.
+      do 31! (rewrite {1} Map.get_set_neqE; first by smt (PurePrimops.add_neq_of_lt)).
+      rewrite Map.get_set_neqE.
+      apply neq_of_lt.
+      exact h_idx2.
+      rewrite h_mem.
+      reflexivity.
+  qed.
+
+lemma mstore_spec:
+    forall (memory: mem) (idx': uint256) (val': uint256),
+hoare [ Primops.mstore :
+    arg = (idx', val') /\
+    Primops.memory = memory ==>
+      Primops.memory = PurePrimops.mstore memory idx' val'
+    ].
+    proof.
+      progress.
+      proc.
+      wp.
+      skip.
+    move => &hr h_args.
+      have h_idx: idx{hr} = idx'.
+      smt.
+      have h_val: val{hr} = val'.
+      smt.
+      have h_mem: Primops.memory{hr} = memory.
+      smt.
+    move => x248 x240 x232 x224 x216 x208 x200 x192 x184 x176 x168 x160 x152 x144 x136 x128 x120 x112 x104 x96 x88 x80 x72 x64 x56 x48 x40 x32 x24 x16 x8.
+      apply PurePrimops.mstore_of_load_and_frame.
+      rewrite h_mem.
+      rewrite /mload.
+      rewrite h_idx.
+      rewrite {1} Map.get_set_sameE.
+      rewrite {1} get_set_offsets_neq; first trivial.
+      rewrite {1} Map.get_set_sameE.
+      rewrite masklsb_zero.
+      rewrite splitMask_zero.
+      rewrite shr_zero.
+      rewrite /x8.
+      rewrite splitMask2_shr_shl; first trivial.
+      rewrite splitMask_add.
+      do 2! (rewrite {1} get_set_offsets_neq; first trivial).
+      rewrite {1} Map.get_set_sameE.
+      rewrite /x16.
+      rewrite splitMask2_shr_shl; first trivial.
+      rewrite splitMask_add.
+      do 3! (rewrite {1} get_set_offsets_neq; first trivial).
+      rewrite {1} Map.get_set_sameE.
+      rewrite /x24.
+      rewrite splitMask2_shr_shl; first trivial.
+      rewrite splitMask_add.    
+      do 4! (rewrite {1} get_set_offsets_neq; first trivial).
+      rewrite {1} Map.get_set_sameE.
+      rewrite /x32.
+      rewrite splitMask2_shr_shl; first trivial.
+      rewrite splitMask_add.    
+      do 5! (rewrite {1} get_set_offsets_neq; first trivial).
+      rewrite {1} Map.get_set_sameE.
+      rewrite /x40.
+      rewrite splitMask2_shr_shl; first trivial.
+      rewrite splitMask_add.    
+      do 6! (rewrite {1} get_set_offsets_neq; first trivial).
+      rewrite {1} Map.get_set_sameE.
+      rewrite /x48.
+      rewrite splitMask2_shr_shl; first trivial.
+      rewrite splitMask_add.
+      do 7! (rewrite {1} get_set_offsets_neq; first trivial).
+      rewrite {1} Map.get_set_sameE.
+      rewrite /x56.
+      rewrite splitMask2_shr_shl; first trivial.
+      rewrite splitMask_add.
+      do 8! (rewrite {1} get_set_offsets_neq; first trivial).
+      rewrite {1} Map.get_set_sameE.
+      rewrite /x64.
+      rewrite splitMask2_shr_shl; first trivial.
+      rewrite splitMask_add.
+      do 9! (rewrite {1} get_set_offsets_neq; first trivial).
+      rewrite {1} Map.get_set_sameE.
+      rewrite /x72.
+      rewrite splitMask2_shr_shl; first trivial.
+      rewrite splitMask_add.
+      do 10! (rewrite {1} get_set_offsets_neq; first trivial).
+      rewrite {1} Map.get_set_sameE.
+      rewrite /x80.
+      rewrite splitMask2_shr_shl; first trivial.
+      rewrite splitMask_add.
+      do 11! (rewrite {1} get_set_offsets_neq; first trivial).
+      rewrite {1} Map.get_set_sameE.
+      rewrite /x88.
+      rewrite splitMask2_shr_shl; first trivial.
+      rewrite splitMask_add.
+      do 12! (rewrite {1} get_set_offsets_neq; first trivial).
+      rewrite {1} Map.get_set_sameE.
+      rewrite /x96.
+      rewrite splitMask2_shr_shl; first trivial.
+      rewrite splitMask_add.
+      do 13! (rewrite {1} get_set_offsets_neq; first trivial).
+      rewrite {1} Map.get_set_sameE.
+      rewrite /x104.
+      rewrite splitMask2_shr_shl; first trivial.
+      rewrite splitMask_add.
+      do 14! (rewrite {1} get_set_offsets_neq; first trivial).
+      rewrite {1} Map.get_set_sameE.
+      rewrite /x112.
+      rewrite splitMask2_shr_shl; first trivial.
+      rewrite splitMask_add.
+      do 15! (rewrite {1} get_set_offsets_neq; first trivial).
+      rewrite {1} Map.get_set_sameE.
+      rewrite /x120.
+      rewrite splitMask2_shr_shl; first trivial.
+      rewrite splitMask_add.
+      do 16! (rewrite {1} get_set_offsets_neq; first trivial).
+      rewrite {1} Map.get_set_sameE.
+      rewrite /x128.
+      rewrite splitMask2_shr_shl; first trivial.
+      rewrite splitMask_add.
+      do 17! (rewrite {1} get_set_offsets_neq; first trivial).
+      rewrite {1} Map.get_set_sameE.
+      rewrite /x136.
+      rewrite splitMask2_shr_shl; first trivial.
+      rewrite splitMask_add.
+      do 18! (rewrite {1} get_set_offsets_neq; first trivial).
+      rewrite {1} Map.get_set_sameE.
+      rewrite /x144.
+      rewrite splitMask2_shr_shl; first trivial.
+      rewrite splitMask_add.
+      do 19! (rewrite {1} get_set_offsets_neq; first trivial).
+      rewrite {1} Map.get_set_sameE.
+      rewrite /x152.
+      rewrite splitMask2_shr_shl; first trivial.
+      rewrite splitMask_add.
+      do 20! (rewrite {1} get_set_offsets_neq; first trivial).
+      rewrite {1} Map.get_set_sameE.
+      rewrite /x160.
+      rewrite splitMask2_shr_shl; first trivial.
+      rewrite splitMask_add.
+      do 21! (rewrite {1} get_set_offsets_neq; first trivial).
+      rewrite {1} Map.get_set_sameE.
+      rewrite /x168.
+      rewrite splitMask2_shr_shl; first trivial.
+      rewrite splitMask_add.
+      do 22! (rewrite {1} get_set_offsets_neq; first trivial).
+      rewrite {1} Map.get_set_sameE.
+      rewrite /x176.
+      rewrite splitMask2_shr_shl; first trivial.
+      rewrite splitMask_add.
+      do 23! (rewrite {1} get_set_offsets_neq; first trivial).
+      rewrite {1} Map.get_set_sameE.
+      rewrite /x184.
+      rewrite splitMask2_shr_shl; first trivial.
+      rewrite splitMask_add.
+      do 24! (rewrite {1} get_set_offsets_neq; first trivial).
+      rewrite {1} Map.get_set_sameE.
+      rewrite /x192.
+      rewrite splitMask2_shr_shl; first trivial.
+      rewrite splitMask_add.
+      do 25! (rewrite {1} get_set_offsets_neq; first trivial).
+      rewrite {1} Map.get_set_sameE.
+      rewrite /x200.
+      rewrite splitMask2_shr_shl; first trivial.
+      rewrite splitMask_add.
+      do 26! (rewrite {1} get_set_offsets_neq; first trivial).
+      rewrite {1} Map.get_set_sameE.
+      rewrite /x208.
+      rewrite splitMask2_shr_shl; first trivial.
+      rewrite splitMask_add.
+      do 27! (rewrite {1} get_set_offsets_neq; first trivial).
+      rewrite {1} Map.get_set_sameE.
+      rewrite /x216.
+      rewrite splitMask2_shr_shl; first trivial.
+      rewrite splitMask_add.
+      do 28! (rewrite {1} get_set_offsets_neq; first trivial).
+      rewrite {1} Map.get_set_sameE.
+      rewrite /x224.
+      rewrite splitMask2_shr_shl; first trivial.
+      rewrite splitMask_add.
+      do 29! (rewrite {1} get_set_offsets_neq; first trivial).
+      rewrite {1} Map.get_set_sameE.
+      rewrite /x232.
+      rewrite splitMask2_shr_shl; first trivial.
+      rewrite splitMask_add.
+      do 30! (rewrite {1} get_set_offsets_neq; first trivial).
+      rewrite {1} Map.get_set_sameE.
+      rewrite /x240.
+      rewrite splitMask2_shr_shl; first trivial.
+      rewrite splitMask_add.
+      do 31! (rewrite {1} get_set_offset; first trivial).
+      rewrite {1} Map.get_set_sameE.
+      rewrite /x248.
+      rewrite splitMask2_shr_shl; first trivial.
+      rewrite splitMask_add.
+      exact h_val.
+      rewrite /uint256_frame.
+    move => idx2 h_idx2.
+      rewrite h_idx.
+      do 31! (rewrite {1} Map.get_set_neqE; first by smt (PurePrimops.add_neq_of_lt)).
+      rewrite Map.get_set_neqE.
+      apply neq_of_lt.
+      exact h_idx2.
+      rewrite h_mem.
+      reflexivity.
+  qed.
+
+
+end ConcretePrimops.
