src/zksync_verifier.ec
@@ -1,31 +1,64 @@
 pragma Goals:printall.
 
-require import Logic UInt256 Memory YulPrimops Array.
+require import Array.
+require import Logic.
+require import Memory.
+require import PurePrimops.
+require import Real.
+require import UInt256.
 require import Utils.
+require import YulPrimops.
 
-op p = W256.of_int 21888242871839275222246405745257275088696311157297823662689037894645226208583.
+op p_int = 21888242871839275222246405745257275088696311157297823662689037894645226208583.
+op p_uint256 = W256.of_int p_int.
 
 module Test = {
-    proc pointNegate(point : uint256) : unit = {
-      var _1, _2, _3, pY, tmp166, tmp167, tmp168, _6, _7;
-      _1 <- W256.of_int 32;
-      _2 <- point + _1;
-      tmp166 <@ Primops.mload(_2);
-      pY <- tmp166;
-      tmp167 <- pY;
-      if (tmp167 = W256.of_int 0)
+
+    proc usr_revertWithMessage(usr_len : uint256, usr_reason : uint256): unit = {
+    var _1, _2, _3, _4, _5, _6, _7;
+    _1 <- (PurePrimops.shl (W256.of_int 229) (W256.of_int 4594637));
+    _2 <- (W256.of_int 0);
+    Primops.mstore(_2, _1);
+    _3 <- (W256.of_int 32);
+    _4 <- (W256.of_int 4);
+    Primops.mstore(_4, _3);
+    _5 <- (W256.of_int 36);
+    Primops.mstore(_5, usr_len);
+    _6 <- (W256.of_int 68);
+    Primops.mstore(_6, usr_reason);
+    _7 <- (W256.of_int 100);
+    Primops.revert(_2, _7);
+    }
+
+  proc usr_pointNegate(usr_point : uint256): unit = {
+    var _1, _2, usr_pY, tmp88, tmp89, _3, tmp90, _4, _5, tmp91, _6, _7;
+    _1 <- (W256.of_int 32);
+    _2 <- (usr_point + _1);
+    tmp88 <@ Primops.mload(_2);
+    usr_pY <- tmp88;
+    tmp89 <- usr_pY;
+    if ((tmp89 = (W256.of_int 0)))
       {
-        tmp168 <@ Primops.mload(point);
-        _3 <- tmp168;
-        if (_3 = W256.of_int 0)
+      tmp90 <@ Primops.mload(usr_point);
+      _3 <- tmp90;
+      if (bool_of_uint256 _3)
         {
-          Primops.revert();
+        _4 <- PurePrimops.STRING (*pointNegate: invalid point*);
+        _5 <- (W256.of_int 26);
+        tmp91 <@ usr_revertWithMessage(_5, _4);
+
         }
-      } else {
-          _6 <- W256.of_int 21888242871839275222246405745257275088696311157297823662689037894645226208583;
-          _7 <- _6 - pY;
-          Primops.mstore(_2, _7);
+
+
       }
+
+    else {
+      _6 <- (W256.of_int 21888242871839275222246405745257275088696311157297823662689037894645226208583);
+      _7 <- (_6 - usr_pY);
+      Primops.mstore(_2, _7);
+
+      }
+
     }
 
     proc writeReadTest(address: uint256, value: uint256): uint256 = {
@@ -34,247 +67,246 @@ module Test = {
       _1 <@ Primops.mload(address);
       return _1;
     }
-}.
+  }.
 
-(* Functional correctness *)
+    (* Functional correctness *)
 
 lemma writeReadTest_correctness :
     forall (address value: uint256),
-hoare [ Test.writeReadTest :
+phoare [ Test.writeReadTest :
       arg = (address, value) ==>
-      res = value].
+      res = value] = 1%r.
 proof.
     progress.
-    proc.
-    inline Primops.mstore Primops.mload.
-    wp.
-    skip.
-    move => &hr hr_eq.
-    move => x248 x240 x232 x224 x216 x208 x200 x192 x184 x176 x168 x160 x152 x144 x136 x128 x120 x112 x104 x96 x88 x80 x72 x64 x56 x48 x40 x32 x24 x16 x8.
-    move => memory.
-    rewrite {1} /memory.
-    rewrite Map.get_set_sameE.
-    rewrite {1} /memory.
-    rewrite get_set_offsets_neq; first trivial.
-    rewrite Map.get_set_sameE.
-    rewrite masklsb_zero.
-    rewrite shr_zero.
-    rewrite splitMask_zero.
-    rewrite /x8.
-    rewrite splitMask2_shr_shl; first trivial.
-    rewrite splitMask_add.
-    rewrite {1} /memory.
-    do 2! (rewrite get_set_offsets_neq; first trivial).
-    rewrite Map.get_set_sameE.
-    rewrite /x128.
-    rewrite splitMask2_shr_shl; first trivial.
-    rewrite splitMask_add.
-    rewrite {1} /memory.
-    do 3! (rewrite get_set_offsets_neq; first trivial).
-    rewrite Map.get_set_sameE.
-    rewrite /x128.
-    rewrite splitMask2_shr_shl; first trivial.
-    rewrite splitMask_add.
-    rewrite {1} /memory.
-    do 4! (rewrite get_set_offsets_neq; first trivial).
-    rewrite Map.get_set_sameE.
-    rewrite /x128.
-    rewrite splitMask2_shr_shl; first trivial.
-    rewrite splitMask_add.
-    rewrite {1} /memory.
-    do 5! (rewrite get_set_offsets_neq; first trivial).
-    rewrite Map.get_set_sameE.
-    rewrite /x128.
-    rewrite splitMask2_shr_shl; first trivial.
-    rewrite splitMask_add.
-    rewrite {1} /memory.
-    do 6! (rewrite get_set_offsets_neq; first trivial).
-    rewrite Map.get_set_sameE.
-    rewrite /x128.
-    rewrite splitMask2_shr_shl; first trivial.
-    rewrite splitMask_add.
-    rewrite {1} /memory.
-    do 7! (rewrite get_set_offsets_neq; first trivial).
-    rewrite Map.get_set_sameE.
-    rewrite /x128.
-    rewrite splitMask2_shr_shl; first trivial.
-    rewrite splitMask_add.
-    rewrite {1} /memory.
-    do 8! (rewrite get_set_offsets_neq; first trivial).
-    rewrite Map.get_set_sameE.
-    rewrite /x128.
-    rewrite splitMask2_shr_shl; first trivial.
-    rewrite splitMask_add.
-    rewrite {1} /memory.
-    do 9! (rewrite get_set_offsets_neq; first trivial).
-    rewrite Map.get_set_sameE.
-    rewrite /x128.
-    rewrite splitMask2_shr_shl; first trivial.
-    rewrite splitMask_add.
-    rewrite {1} /memory.
-    do 10! (rewrite get_set_offsets_neq; first trivial).
-    rewrite Map.get_set_sameE.
-    rewrite /x128.
-    rewrite splitMask2_shr_shl; first trivial.
-    rewrite splitMask_add.
-    rewrite {1} /memory.
-    do 11! (rewrite get_set_offsets_neq; first trivial).
-    rewrite Map.get_set_sameE.
-    rewrite /x128.
-    rewrite splitMask2_shr_shl; first trivial.
-    rewrite splitMask_add.
-    rewrite {1} /memory.
-    do 12! (rewrite get_set_offsets_neq; first trivial).
-    rewrite Map.get_set_sameE.
-    rewrite /x128.
-    rewrite splitMask2_shr_shl; first trivial.
-    rewrite splitMask_add.
-    rewrite {1} /memory.
-    do 13! (rewrite get_set_offsets_neq; first trivial).
-    rewrite Map.get_set_sameE.
-    rewrite /x128.
-    rewrite splitMask2_shr_shl; first trivial.
-    rewrite splitMask_add.
-    rewrite {1} /memory.
-    do 14! (rewrite get_set_offsets_neq; first trivial).
-    rewrite Map.get_set_sameE.
-    rewrite /x128.
-    rewrite splitMask2_shr_shl; first trivial.
-    rewrite splitMask_add.
-    rewrite {1} /memory.
-    do 15! (rewrite get_set_offsets_neq; first trivial).
-    rewrite Map.get_set_sameE.
-    rewrite /x128.
-    rewrite splitMask2_shr_shl; first trivial.
-    rewrite splitMask_add.
-    rewrite {1} /memory.
-    do 16! (rewrite get_set_offsets_neq; first trivial).
-    rewrite Map.get_set_sameE.
-    rewrite /x128.
-    rewrite splitMask2_shr_shl; first trivial.
-    rewrite splitMask_add.
-    rewrite {1} /memory.
-    do 17! (rewrite get_set_offsets_neq; first trivial).
-    rewrite Map.get_set_sameE.
-    rewrite /x136.
-    rewrite splitMask2_shr_shl. trivial.
-    rewrite splitMask_add.
-    rewrite {1} /memory.
-    do 18! (rewrite get_set_offsets_neq; first trivial).
-    rewrite Map.get_set_sameE.
-    rewrite /x144.
-    rewrite splitMask2_shr_shl. trivial.
-    rewrite splitMask_add.
-    rewrite {1} /memory.
-    do 19! (rewrite get_set_offsets_neq; first trivial).
-    rewrite Map.get_set_sameE.
-    rewrite /x152.
-    rewrite splitMask2_shr_shl. trivial.
-    rewrite splitMask_add.
-    rewrite {1} /memory.
-    do 20! (rewrite get_set_offsets_neq; first trivial).
-    rewrite Map.get_set_sameE.
-    rewrite /x160.
-    rewrite splitMask2_shr_shl. trivial.
-    rewrite splitMask_add.
-    rewrite {1} /memory.
-    do 21! (rewrite get_set_offsets_neq; first trivial).
-    rewrite Map.get_set_sameE.
-    rewrite /x168.
-    rewrite splitMask2_shr_shl. trivial.
-    rewrite splitMask_add.
-    rewrite {1} /memory.
-    do 22! (rewrite get_set_offsets_neq; first trivial).
-    rewrite Map.get_set_sameE.
-    rewrite /x176.
-    rewrite splitMask2_shr_shl. trivial.
-    rewrite splitMask_add.
-    rewrite {1} /memory.
-    do 23! (rewrite get_set_offsets_neq; first trivial).
-    rewrite Map.get_set_sameE.
-    rewrite /x184.
-    rewrite splitMask2_shr_shl. trivial.
-    rewrite splitMask_add.
-    rewrite {1} /memory.
-    do 24! (rewrite get_set_offsets_neq; first trivial).
-    rewrite Map.get_set_sameE.
-    rewrite /x192.
-    rewrite splitMask2_shr_shl. trivial.
-    rewrite splitMask_add.
-    rewrite {1} /memory.
-    do 25! (rewrite get_set_offsets_neq; first trivial).
-    rewrite Map.get_set_sameE.
-    rewrite /x200.
-    rewrite splitMask2_shr_shl. trivial.
-    rewrite splitMask_add.
-    rewrite {1} /memory.
-    do 26! (rewrite get_set_offsets_neq; first trivial).
-    rewrite Map.get_set_sameE.
-    rewrite /x208.
-    rewrite splitMask2_shr_shl. trivial.
-    rewrite splitMask_add.
-    rewrite {1} /memory.
-    do 27! (rewrite get_set_offsets_neq; first trivial).
-    rewrite Map.get_set_sameE.
-    rewrite /x216.
-    rewrite splitMask2_shr_shl. trivial.
-    rewrite splitMask_add.
-    rewrite {1} /memory.
-    do 28! (rewrite get_set_offsets_neq; first trivial).
-    rewrite Map.get_set_sameE.
-    rewrite /x224.
-    rewrite splitMask2_shr_shl. trivial.
-    rewrite splitMask_add.
-    rewrite {1} /memory.
-    do 29! (rewrite get_set_offsets_neq; first trivial).
-    rewrite Map.get_set_sameE.
-    rewrite /x232.
-    rewrite splitMask2_shr_shl. trivial.
-    rewrite splitMask_add.
-    rewrite {1} /memory.
-    do 30! (rewrite get_set_offsets_neq; first trivial).
-    rewrite Map.get_set_sameE.
-    rewrite /x240.
-    rewrite splitMask2_shr_shl. trivial.
-    rewrite splitMask_add.
-    rewrite {1} /memory.
-    do 31! (rewrite get_set_offset; first trivial).
-    rewrite Map.get_set_sameE.
-    rewrite /x248.
-    rewrite splitMask2_shr_shl; first trivial.
-    rewrite splitMask_add.
-    have injection: forall (a b c d: uint256), (a, b) = (c, d) => b = d.
-    progress.
-    smt.
+  proc.
+  exists* Primops.memory.
+  elim*=>memory_pre.
+  call (ConcretePrimops.mload_pspec (PurePrimops.mstore memory_pre address value) address).
+  call (ConcretePrimops.mstore_pspec memory_pre address value).
+  skip.
+  progress.
+  apply PurePrimops.mload_mstore_same.
 qed.
-      
-lemma pointNegate_correctness :
-    forall (x y point_addr : uint256),
-hoare [ Test.pointNegate :
-    arg = point_addr /\
-    (x <> W256.zero \/ y <> W256.zero) /\
-        Primops.memory.[point_addr] = x /\
-        Primops.memory.[point_addr + (W256.of_int 32)] = y /\
-        y < p ==>
-    (
-        Primops.reverted = false =>
-    (
-        Primops.memory.[point_addr] = x /\
-        Primops.memory.[point_addr + (W256.of_int 32)] = (-y) %% p
-    )
-)]. proof.
-    progress.
+
+lemma usr_revertWithMessage_correctness :
+    forall (size reason : uint256),
+hoare [ Test.usr_revertWithMessage :
+      arg = (size, reason) ==>
+    Primops.reverted = true
+    ].
+    proof.
+      progress.
+      proc.
+      inline Primops.mload Primops.mstore Primops.revert.
+      wp.
+      skip.
+      progress.
+  qed.
+
+  type Point = int * int.
+  op NegatePoint (point: Point): Point = (point.`1, (-point.`2) %% p_int).
+  op IsPointWellformed (point: Point): bool = 0 <= point.`1 /\ 0 <= point.`2 /\ point.`1 < p_int /\ point.`2 < p_int.
+  op IsPointValid (point: Point): bool = !(point.`1 <> 0 /\ point.`2 = 0).
+
+module PointNegate = {
+  proc low(point: uint256) : unit = {
+    var x, y;
+    x <@ Primops.mload(point);
+    y <@ Primops.mload(point + W256.of_int 32);
+    if (y <> W256.zero) {
+        Primops.mstore(point + W256.of_int 32, p_uint256 - y);
+    }
+    
+    if (x <> W256.zero /\ y = W256.zero) {
+      Primops.revert(W256.zero, W256.zero);
+    }
+  }
+
+  proc mid(point_x: int, point_y: int) : int * int = {
+    var ret_x, ret_y;
+    ret_x <- point_x;
+    ret_y <- (-point_y) %% p_int;
+
+    if (point_x <> 0 /\ point_y = 0) {
+      Primops.reverted <- true;
+    }
+
+    return (ret_x, ret_y);
+  }
+
+      proc high(point: Point): Point = {
+    (* option instead of revert *)
+    if (!IsPointValid point) {
+      Primops.reverted <- true;
+    }
+
+    return (NegatePoint point);
+  }
+}.
+
+lemma pointNegate_actual_matches_low: equiv [
+    Test.usr_pointNegate ~ PointNegate.low :
+    Primops.memory{1} = Primops.memory{2} /\
+      arg{1} = arg{2} /\
+    !Primops.reverted{1} /\
+    !Primops.reverted{2}
+      ==>
+        Primops.reverted{1} <=> Primops.reverted{2} /\
+        (!Primops.reverted{1}) =>
+        forall (idx: uint256),
+        Primops.memory{1}.[idx] =
+        Primops.memory{2}.[idx]
+    ].
+    proof.
+      exists* Primops.memory{1}.
+      elim*=>memory.
+      exists* usr_point{1}.
+      elim*=>point.
+      proc.
+      case (PurePrimops.mload memory (point+W256.of_int 32) = W256.zero). (* case y=0 *)
+      rcondt{1} 6; first last.                                                   (* actual: take the no-writing branch *)
+      rcondf{2} 3; first last.                                                   (* low: take the no-writing branch *)
+      case (PurePrimops.mload memory point = W256.zero).                     (* case x=0 *)
+      rcondf{1} 8; first last.                                                     (* actual: take the non-reverting branch *)
+      rcondf{2} 3; first last.                                                     (* low: take the non-reverting branch *)
+      sim.                                                                         (* simplify post to just equating memory *)
+      inline Primops.mload.
+      by sim.                                                                         (* prove memory is unchanged *)
+      progress.                                                                    (* to prove: x and y are loaded correctly in the low spec *)
+      call (ConcretePrimops.mload_spec memory (point + W256.of_int 32)).           (* load y *)
+      call (ConcretePrimops.mload_spec memory point).                              (* load x *)
+      skip.
+      progress.
+      rewrite H2 H1.
+      by trivial.
+      progress.                                                                    (* to prove: x is loaded correctly in actual *)
+      wp.
+      call (ConcretePrimops.mload_spec memory point).                              (* load x *)
+      inline Primops.mload. wp. skip. by progress.                                    (* discharge the rest of the program *)
+                                                                                 (* case x <> 0 *)
+      rcondt{1} 8; first last.                                                     (* actual: take the reverting branch *)
+      rcondt{2} 3; first last.                                                     (* low: take the reverting branch *)
+      inline Test.usr_revertWithMessage Primops.revert Primops.mstore Primops.mload. (* sim here breaks the proof *)
+      wp. skip. by progress.
+      progress.                                                                    (* to prove: x and y are loaded correctly in the low spec *)
+      call (ConcretePrimops.mload_spec memory (point + W256.of_int 32)).           (* load y *)
+      call (ConcretePrimops.mload_spec memory point).                              (* load x *)
+      skip. by progress.
+      progress.                                                                    (* to prove: x loaded correct in actual *)
+      wp.
+      call (ConcretePrimops.mload_spec memory point).   
+      inline Primops.mload. wp. skip. by progress.
+      progress.                                                                  (* to prove: y loaded correctly in low *)
+      call (ConcretePrimops.mload_spec memory (point + W256.of_int 32)).
+      inline Primops.mload. wp. skip. by progress.
+      progress.                                                                  (* to prove: y loaded correctly in actual *)
+      wp.                                                                         
+      call (ConcretePrimops.mload_spec memory (point + W256.of_int 32)).         
+      wp. skip. by progress.                                                     
+                                                                             (* case y<>0 *)
+      rcondf{1} 6; first last.                                                 (* actual: take writing branch *)
+      rcondf{2} 4; first last.                                                 (* low: skip reverting branch *)
+      rcondt{2} 3; first last.                                                 (* low: take writing branch *)
+      sim. inline Primops.mstore Primops.mload. wp. skip. by progress.         (* prove that neither revert and memory maps are modified equally *)
+      progress.                                                                (* prove that y is loaded correct in low *)
+      call (ConcretePrimops.mload_spec memory (point + W256.of_int 32)).
+      inline Primops.mload. wp. skip. by progress.
+      progress.                                                                (* prove that x and y are loaded correct in low and the writing branch is taken *)
+      rcondt 3; first last.                                                    (* take the writing branch *)
+      inline Primops.mstore. wp.
+      call (ConcretePrimops.mload_spec memory (point + W256.of_int 32)).
+      call (ConcretePrimops.mload_spec memory point).
+      skip. progress. rewrite H1. by trivial.
+      call (ConcretePrimops.mload_spec memory (point + W256.of_int 32)).
+      inline Primops.mload. wp. skip. by progress.
+      progress.                                                                (* prove y is loaded correctly in actual *)
+      wp.
+      call (ConcretePrimops.mload_spec memory (point + W256.of_int 32)).
+      wp. skip. by progress.
+  qed.
+
+lemma zero_of_to_uint_zero (x: uint256): to_uint x = 0 => x = W256.zero.
+    proof.
+      by smt(@W256).
+    qed.
+
+lemma pointNegate_low_matches_mid (memory: mem) (point_address: uint256) (point_x_int point_y_int: int): equiv [
+    PointNegate.low ~ PointNegate.mid :
+      arg{2} = (point_x_int, point_y_int) /\
+      arg{1} = point_address /\
+      Primops.memory{1} = memory /\
+      W256.to_uint(PurePrimops.mload memory point_address) = point_x_int /\
+      W256.to_uint(PurePrimops.mload memory (point_address + W256.of_int 32)) = point_y_int /\
+      !Primops.reverted{1} /\
+      !Primops.reverted{2}
+      ==>
+        Primops.reverted{1} <=> Primops.reverted{2} /\ (
+        (!Primops.reverted{1}) => (
+          Primops.memory{1} = PurePrimops.mstore (PurePrimops.mstore memory point_address (W256.of_int res{2}.`1)) (point_address + W256.of_int 32) (W256.of_int res{2}.`2)
+        ))
+    ].
+    proof.
+      exists* Primops.memory{1}.
+      elim*=> memory_pre.
+      proc.
+    case (point_y_int = 0).
+      rcondf{1} 3. progress.
+      call (ConcretePrimops.mload_spec memory (point_address + W256.of_int 32)).
+      call (ConcretePrimops.mload_spec memory point_address).
+      skip. progress.
+      apply zero_of_to_uint_zero. exact H1.
+    case (point_x_int = 0).
+      rcondf{1} 3. progress.
+      call (ConcretePrimops.mload_spec memory (point_address + W256.of_int 32)).
+      call (ConcretePrimops.mload_spec memory point_address).
+      skip. progress.
+      by smt (zero_of_to_uint_zero).
+      rcondf{2} 3. progress.
+      wp. skip. progress.
+      by smt (zero_of_to_uint_zero).
+      wp.
+      kill{1} 0 ! 2; first (inline Primops.mload; wp; skip; by progress).
+      skip.
+      by progress.
+      (* case point_x_int <> 0 *)
+      rcondt{1} 3. progress.
+      call (ConcretePrimops.mload_spec memory (point_address + W256.of_int 32)).
+      call (ConcretePrimops.mload_spec memory point_address).
+      skip. progress; by smt (@W256).
+      rcondt{2} 3. progress.
+      wp. skip. by progress.
+      inline Primops.revert.
+      kill{1} 0 ! 4. inline Primops.mload. wp. skip. by progress.
+      wp. skip. by progress.
+      (* case point_y_int <> 0 *)
+      rcondt{1} 3. progress.
+      call (ConcretePrimops.mload_spec memory (point_address + W256.of_int 32)).
+      call (ConcretePrimops.mload_spec memory point_address).
+      skip. progress. by smt (@W256).
+      rcondf{1} 4. progress.
+      inline Primops.mstore. wp.
+      call (ConcretePrimops.mload_spec memory (point_address + W256.of_int 32)).
+      call (ConcretePrimops.mload_spec memory point_address).
+      skip. progress. by smt (@W256).
+      rcondf{2} 3. progress. wp. skip. progress. by smt (@W256).
+      call{1} (ConcretePrimops.mstore_pspec memory_pre (point_address + W256.of_int 32) (p_uint256 - W256.of_int point_y_int)).
+      call{1} (ConcretePrimops.mload_pspec memory_pre (point_address + W256.of_int 32)).
+      call{1} (ConcretePrimops.mload_pspec memory_pre point_address).
+      wp. skip. by progress.
+    qed.
+    
+lemma pointNegate_mid_matches_high (point: Point):
+  equiv [
+    PointNegate.mid ~ PointNegate.high :
+      arg{2} = (arg{1}.`1, arg{1}.`2) /\
+      arg{2} = point /\
+    IsPointWellformed point /\
+    !Primops.reverted{1} /\
+      !Primops.reverted{2}
+      ==>
+    (Primops.reverted{1} <=> Primops.reverted{2}) /\ (!Primops.reverted{1} => res{2} = (res{1}.`1, res{1}.`2))
+  ].
+  proof.
     proc.
-    simplify.
-    inline Primops.mload Primops.mstore Primops.revert.
-    wp.
-    skip.
-    progress.
-    rewrite H1.
-    admit.
-    rewrite Map.get_set_neqE.
-    admit.
-    auto.
-    rewrite Map.get_set_sameE.
-    admit.
+    wp. skip. progress; by smt().
 qed.
