src/PurePrimops.ec
@@ -1,0 +1,223 @@
+pragma Goals:printall.
+
+require import Array.
+require import Logic.
+require import Memory.
+require export UInt256.
+require import Utils.
+
+theory PurePrimops.
+
+(* definitions ========== *)
+
+op calldata : uint256 array.
+op keccak256_f : uint256 array -> uint256.
+
+op iszero(v : uint256) : uint256 = if (v = W256.zero) then W256.one else  W256.zero.
+
+op mload (memory: mem) (idx: uint256) =
+    memory.[idx+ W256.of_int 31] +
+    (memory.[idx+ W256.of_int 30] `<<<` 8) +
+    (memory.[idx+ W256.of_int 29] `<<<` 16) +
+    (memory.[idx+ W256.of_int 28] `<<<` 24) +
+    (memory.[idx+ W256.of_int 27] `<<<` 32) +
+    (memory.[idx+ W256.of_int 26] `<<<` 40) +
+    (memory.[idx+ W256.of_int 25] `<<<` 48) +
+    (memory.[idx+ W256.of_int 24] `<<<` 56) +
+    (memory.[idx+ W256.of_int 23] `<<<` 64) +
+    (memory.[idx+ W256.of_int 22] `<<<` 72) +
+    (memory.[idx+ W256.of_int 21] `<<<` 80) +
+    (memory.[idx+ W256.of_int 20] `<<<` 88) +
+    (memory.[idx+ W256.of_int 19] `<<<` 96) +
+    (memory.[idx+ W256.of_int 18] `<<<` 104) +
+    (memory.[idx+ W256.of_int 17] `<<<` 112) +
+    (memory.[idx+ W256.of_int 16] `<<<` 120) +
+    (memory.[idx+ W256.of_int 15] `<<<` 128) +
+    (memory.[idx+ W256.of_int 14] `<<<` 136) +
+    (memory.[idx+ W256.of_int 13] `<<<` 144) +
+    (memory.[idx+ W256.of_int 12] `<<<` 152) +
+    (memory.[idx+ W256.of_int 11] `<<<` 160) +
+    (memory.[idx+ W256.of_int 10] `<<<` 168) +
+    (memory.[idx+ W256.of_int 9] `<<<` 176) +
+    (memory.[idx+ W256.of_int 8] `<<<` 184) +
+    (memory.[idx+ W256.of_int 7] `<<<` 192) +
+    (memory.[idx+ W256.of_int 6] `<<<` 200) +
+    (memory.[idx+ W256.of_int 5] `<<<` 208) +
+    (memory.[idx+ W256.of_int 4] `<<<` 216) +
+    (memory.[idx+ W256.of_int 3] `<<<` 224) +
+    (memory.[idx+ W256.of_int 2] `<<<` 232) +
+    (memory.[idx+ W256.of_int 1] `<<<` 240) +
+    (memory.[idx] `<<<` 248)
+    axiomatized by mLoadE.
+
+op mstore (memory: mem) (idx val: uint256): mem.
+
+op mulmod(a b n : uint256) : uint256 =
+  let a_int = W256.to_uint a in
+  let b_int = W256.to_uint b in
+  let n_int = W256.to_uint n in
+  W256.of_int ((a_int * b_int) %% n_int)
+axiomatized by mulmodE.
+
+op addmod(a b n : uint256) : uint256 =
+  let a_int = W256.to_uint a in
+  let b_int = W256.to_uint b in
+  let n_int = W256.to_uint n in
+  W256.of_int ((a_int + b_int) %% n_int)
+axiomatized by addmodE.
+
+op bit_and(a : uint256, b : uint256) : uint256 = a `&` b
+axiomatized by bit_andE.
+
+op shl(a : uint256, b : uint256) : uint256 = a `<<<` (W256.to_uint b)
+axiomatized by shlE.
+
+op shr(a : uint256, b : uint256) : uint256 = a `>>>` (W256.to_uint b)
+axiomatized by shrE.
+
+op STRING : uint256 = W256.zero.
+
+
+(* lemmas =========== *)
+
+(* iszero *)
+lemma iszero_zeroE : iszero (W256.zero) = W256.one.
+    proof.
+      rewrite /iszero.
+      simplify.
+      trivial.
+  qed.
+lemma iszero_nonzeroE (val: uint256) : val <> W256.zero => iszero val = W256.zero.
+    proof.
+      progress.
+      rewrite /iszero.
+      smt ().
+  qed.
+
+(* mstore *)
+op words_overlap (address1 address2: uint256) =
+  (exists (offset: int), 0 <= offset /\ offset < 32 /\ address1 + W256.of_int offset = address2) \/
+  (exists (offset: int), 0 <= offset /\ offset < 32 /\ address2 + W256.of_int offset = address1)
+  axiomatized by words_overlapE.
+
+lemma subK (a b c: uint256): a - b <> a - c => b <> c.
+    proof.
+      progress.
+      (* smt (@W256). *)
+      smt iterate.
+  qed.
+
+lemma sub_self (a: uint256): a - a = W256.zero.
+    proof.
+      smt (@W256).
+  qed.
+
+lemma sub_add (a b c: uint256): a - (b + c) = a - b - c.
+    proof.
+      smt (@W256).
+  qed.
+
+lemma mod_of_lt (a b: int): 0 < a => 0 < b => a < b => a %% b = a.
+    proof.
+      smt ().
+  qed.
+
+lemma get_right (a b c: int): a <= b < c => b < c.
+    proof.
+      smt().
+    qed.
+
+lemma add_neq_of_lt (idx idx2: uint256) (offset: int):
+    W256.of_int 31 < idx2 - idx =>  0 <= offset /\ offset < 32 => (idx + W256.of_int offset) <> idx2.
+    proof.
+      progress.
+      rewrite W256.ultE W256.of_uintK in H.
+      apply (subK idx2).
+      rewrite sub_self.
+      rewrite sub_add.
+      rewrite /W256.ulift2.
+      have Lifted: W256.of_int (W256.to_uint (idx2 - idx) - offset) <> W256.of_int 0.
+      pose diff := to_uint (idx2 - idx).
+      have diff_gt:  31 < diff.
+      rewrite /diff.
+      rewrite (mod_of_lt 31 W256.modulus) in H; trivial.
+      have diff_lt: diff < W256.modulus.
+      rewrite /diff.
+      exact (get_right 0 (to_uint (idx2 - idx)) W256.modulus (W256.to_uint_cmp (idx2 - idx))).
+      smt (@W256).
+      smt (@W256).
+  qed.
+
+lemma no_overlap (idx idx2: uint256):
+    W256.of_int 31 < idx - idx2 => W256.of_int 31 < idx2 - idx => !words_overlap idx idx2.
+    proof.
+      progress.
+      smt (add_neq_of_lt).
+  qed.
+
+op uint256_frame (memory_pre memory_post: mem) (idx: uint256) = forall (idx2: uint256), W256.of_int 31 < idx2 - idx => memory_post.[idx2] = memory_pre.[idx2].
+
+axiom mload_mstore_same (memory: mem) (idx val: uint256):
+  mload (mstore memory idx val) idx = val.
+
+axiom mstore_frame (memory: mem) (idx val: uint256):
+  uint256_frame memory (mstore memory idx val) idx.
+
+axiom mstore_of_load_and_frame (memory_pre memory_post: mem) (idx val: uint256):
+  mload memory_post idx = val =>
+  uint256_frame memory_pre memory_post idx =>
+  memory_post = mstore memory_pre idx val.
+
+lemma apply_mstore_mload_diff (memory: mem) (idx idx2 val: uint256):
+    W256.of_int 31 < idx2 - idx => W256.of_int 31 < idx - idx2 =>  mload (mstore memory idx val) idx2 = mload memory idx2.
+proof.
+  progress.
+  rewrite /mload.
+  pose memory_post := mstore memory idx val.
+  have h_full: mload memory_post idx = val /\ uint256_frame memory memory_post idx. by smt.
+  have h_frame: uint256_frame memory memory_post idx. smt.
+  rewrite /uint256_frame in h_frame.
+  have h31: forall (offset: int), 0 <= offset => offset < 32 => memory_post.[idx2 + W256.of_int offset] = memory.[idx2 + W256.of_int offset].
+  progress.
+  apply h_frame.
+  rewrite /W256.\ult.
+  rewrite W256.of_uintK.
+  rewrite mod_of_lt; trivial.
+  by smt timeout=10.
+  have h0: memory_post.[idx2] = memory.[idx2] by smt.
+  (rewrite (h31 31); first trivial); first trivial.
+  (rewrite (h31 30); first trivial); first trivial.
+  (rewrite (h31 29); first trivial); first trivial.
+  (rewrite (h31 28); first trivial); first trivial.
+  (rewrite (h31 27); first trivial); first trivial.
+  (rewrite (h31 26); first trivial); first trivial.
+  (rewrite (h31 25); first trivial); first trivial.
+  (rewrite (h31 24); first trivial); first trivial.
+  (rewrite (h31 23); first trivial); first trivial.
+  (rewrite (h31 22); first trivial); first trivial.
+  (rewrite (h31 21); first trivial); first trivial.
+  (rewrite (h31 20); first trivial); first trivial.
+  (rewrite (h31 19); first trivial); first trivial.
+  (rewrite (h31 18); first trivial); first trivial.
+  (rewrite (h31 17); first trivial); first trivial.
+  (rewrite (h31 16); first trivial); first trivial.
+  (rewrite (h31 15); first trivial); first trivial.
+  (rewrite (h31 14); first trivial); first trivial.
+  (rewrite (h31 13); first trivial); first trivial.
+  (rewrite (h31 12); first trivial); first trivial.
+  (rewrite (h31 11); first trivial); first trivial.
+  (rewrite (h31 10); first trivial); first trivial.
+  (rewrite (h31 9); first trivial); first trivial.
+  (rewrite (h31 8); first trivial); first trivial.
+  (rewrite (h31 7); first trivial); first trivial.
+  (rewrite (h31 6); first trivial); first trivial.
+  (rewrite (h31 5); first trivial); first trivial.
+  (rewrite (h31 4); first trivial); first trivial.
+  (rewrite (h31 3); first trivial); first trivial.
+  (rewrite (h31 2); first trivial); first trivial.
+  (rewrite (h31 1); first trivial); first trivial.
+    rewrite h0.
+    reflexivity.
+qed.
+
+end PurePrimops.
